coq/coq/Translation.v
@@ -11,13 +11,164 @@ Import IfNotations.
 Require Export syntax_ott.
 Require Export Infrastructure.
 
-Lemma TEI_dup : forall (ll:string) (At Bt Ct Ct' At':ttyp),
-     rec_typ Ct ->
-      (   (  Tlookup  ll   Ct  = Some  At'   /\  eqIndTypTarget At' At )    \/   Tlookup  ll   Ct  = None  )  ->
-     eqIndTypTarget At Bt ->
-     eqIndTypTarget (ttyp_rcd ll Bt  (ttyp_rcd ll At Ct) ) Ct' ->
-     eqIndTypTarget (ttyp_rcd ll At  (ttyp_rcd ll Bt Ct) ) Ct'.
+(* merge, sort *)
+Lemma HdRel_relax : forall a l,
+    HdRel lex_lt a l -> HdRel NOTF.le a l.
+Proof with eauto.
+  introv HS. induction* HS. constructor...
+  left*.
+Qed.
+
+Definition sorted := Sorted lex_lt.
+
+Theorem sorted_unique : forall (l1 l2 : list string),
+    sorted l1 -> sorted l2 -> Permutation l1 l2 -> l1 = l2.
+Proof.
+  introv HS1 HS2 HP.
+  applys* Sort_In_eq lex_lt.
+  applys lex_lt_trans.
+  applys lex_lt_not_eq.
+  split; introv HI;
+    eauto using Permutation_sym, Permutation_in.
+Qed.
+
+Lemma sorted_relax : forall l,
+    sorted l -> Sorted NOTF.le l.
+Proof with eauto.
+  introv HS. induction* HS.
+  destruct H... constructor... constructor...
+  left*.
+Qed.
+
+#[local] Hint Constructors Sorted HdRel : core.
+#[local] Hint Resolve HdRel_relax sorted_relax : core.
+
+Lemma merge_empty : forall l,
+    merge nil l = l.
+Proof.
+  introv. induction* l.
+Qed.
+
+Lemma merge_empty_r : forall l,
+    merge l nil = l.
+Proof.
+  introv. induction* l.
+Qed.
+
+#[local] Hint Rewrite merge_empty merge_empty_r : merge.
+
+Lemma merge_cons : forall a l b r,
+    merge (a::l) (b::r) =
+      if if proj1_sig (string_compare_lex a b) is Gt then false else true then a :: merge l (b::r) else b :: merge (a::l) r.
+Proof with eauto.
+  introv. induction* l; destruct (proj1_sig (string_compare_lex a b)); autorewrite with merge...
+Qed.
+
+#[local] Hint Rewrite merge_cons : merge.
+
+Lemma test : forall a l r,
+    HdRel NOTF.le a l -> HdRel NOTF.le a r -> HdRel NOTF.le a (merge l r).
 Admitted.
+
+Lemma merge_sorted : forall l r,
+    sorted l -> sorted r -> Sorted NOTF.le (merge l r).
+Proof with eauto using sorted_relax.
+  introv HSl HSr. gen r.
+  induction HSl; intros; autorewrite with merge...
+  - induction HSr...
+    + autorewrite with merge.
+      constructor...
+    + destruct (string_compare_lex a a0) eqn:HE. destruct c.
+      * subst*. simpl. rewrite HE. simpl...
+        econstructor. applys IHHSl...
+        econstructor... applys test...
+        econstructor... right*.
+      * simpl. rewrite HE. simpl...
+        forwards* IH: IHHSl (a0 :: l0)...
+        all: econstructor...
+        applys test...
+      * simpl. rewrite HE. simpl...
+        econstructor... applys test (a :: l) l0...
+Qed.
+
+Lemma HdRel_nodup : forall a l,
+    Sorted NOTF.le l -> HdRel lex_lt a l -> HdRel lex_lt a (nodup string_dec l).
+Proof with eauto.
+  introv HS HR.
+  applys In_InfA. introv HI. apply nodup_In in HI.
+  induction l.
+  - inverts HI.
+  - apply in_inv in HI. destruct HI.
+    + subst*. inverts* HR.
+    + inverts HS. inverts HR.
+      forwards*: IHl.
+      inverts* H3. constructor.
+      destruct H0. now applys* lex_lt_trans.
+      now subst*.
+Qed.
+
+Lemma sorted_nodup : forall l,
+    Sorted NOTF.le l -> sorted (nodup string_dec l).
+Proof with eauto.
+  introv HS. induction* l.
+  - simpl... econstructor...
+  - inverts HS. forwards*: IHl.
+    simpl. case_if.
+    + apply H.
+    + econstructor... destruct l...
+      * simpl...
+      * applys* HdRel_nodup.
+        inverts H2. inverts* H3.
+        exfalso. applys C. applys in_eq.
+Qed.
+
+Lemma merge_sorted_dedup: forall l r,
+    sorted l -> sorted r -> sorted (nodup string_dec (merge l r)).
+Proof with eauto using sorted_nodup, sorted_relax.
+  introv HSl HSr.
+  forwards: merge_sorted HSl HSr...
+Qed.
+
+(* record types *)
+Lemma rcd_typ_concat_simpl : forall T1 T2,
+    rec_typ T1 -> rec_typ T2 ->
+    rec_typ (ttyp_concat_simpl T1 T2).
+Proof with eauto.
+  introv WF1 WF2.
+  induction WF1...
+  - simpl...
+Qed.
+
+Lemma translate_to_record_types : forall A,
+    rec_typ |[ A ]|.
+Proof with eauto using rcd_typ_concat_simpl.
+  introv. induction A; simpl; try case_if; simpl...
+Qed.
+
+#[local] Hint Resolve translate_to_record_types : core.
+
+Lemma lookup_concat_simpl : forall i A B T,
+    Tlookup i A = Some T ->
+    Tlookup i (ttyp_concat_simpl A B) = Tlookup i A.
+Proof.
+  introv LK. gen i T B.
+  induction A; intros; simpl in LK; inverts LK.
+  case_if*.
+  - inverts* H0.
+    subst. simpl. case_if*.
+  - simpl. case_if*.
+Qed.
+
+
+Lemma lookup_concat_simpl_none : forall i A B,
+    Tlookup i A = None -> rec_typ A ->
+    Tlookup i (ttyp_concat_simpl A B) = Tlookup i B.
+Proof.
+  introv LK HR. gen i B.
+  induction A; intros; simpl; try solve_by_invert; eauto.
+  - inverts* HR. inverts LK. case_if.
+    forwards* Heq: IHA2.
+Qed.
 
 Lemma lookup_wf_typ_1 : forall l T At l',
     Tlookup l' (ttyp_rcd l T At) = Tlookup l' At \/ l = l'.
@@ -50,9 +201,20 @@ Qed.
 
 #[local] Hint Resolve lookup_wf_typ_2 lookup_wf_typ_3 wf_typ_look_up_wf : core.
 
+
+Lemma lookup_concat_simpl_destruct : forall l B1 B2,
+    Tlookup l (ttyp_concat_simpl |[ B1 ]| |[ B2 ]|) = Tlookup l |[ B1 ]| \/
+    Tlookup l (ttyp_concat_simpl |[ B1 ]| |[ B2 ]|) = Tlookup l |[ B2 ]|.
+Proof.
+  introv. remember (Tlookup l |[ B1 ]|). destruct o.
+  - forwards* Heq: lookup_concat_simpl  (|[ B1 ]|) (|[ B2 ]|).
+    rewrite Heq. rewrite* <- Heqo.
+  - forwards* Heq: lookup_concat_simpl_none  (|[ B1 ]|) (|[ B2 ]|).
+Qed.
+
 Ltac unify_lookup :=
-      destruct_disj; destruct_conj;
-      repeat lazymatch goal with
+  destruct_disj; destruct_conj;
+  repeat lazymatch goal with
     | |- Some _ = Some _  => try reflexivity
     | H : Some _ = None |- _ => inverts H
     | H : Some _ = Some _ |- _ => inverts H
@@ -67,8 +229,8 @@ Ltac unify_lookup :=
     | H: ?l <> ?r |- Tlookup ?r (ttyp_rcd ?l ?A ?C) = _ => simpl; case_if
     | H: ?r <> ?l |- Tlookup ?r (ttyp_rcd ?l ?A ?C) = _ => simpl; case_if
     | |- Tlookup ?l (ttyp_rcd ?l ?A ?C) = _ => simpl; case_if
-        end.
-
+    | H1: Tlookup _ ?A = Some _ , H2: ?A = ttyp_top |- _ => rewrite H2 in H1; discriminate
+    end.
 
 Ltac destruct_lookup H :=
       match type of H with
@@ -78,11 +240,773 @@ Ltac destruct_lookup H :=
         let Heq := fresh "Heq" in
         lets [Heq|Heq]: lookup_wf_typ_1 l A C r;
         [ rewrite Heq in H; clear Heq | subst ]
+      |  Tlookup _ (ttyp_concat_simpl |[ ?A ]| |[ ?B ]|) = _ =>
+           let Heq := fresh "Heq" in
+           lets [Heq|Heq]: lookup_concat_simpl_destruct A B;
+           rewrite Heq in H
       end.
 
 
-(* TEI eqIndTypTarget *)
-(* #[local] Hint Unfold Tlookup : core. *)
+(* translate *)
+From Ltac2 Require Ltac2.
+
+(** magic from https://coq.discourse.group/t/force-application-of-fixpoint-to-its-argument/1190/8 **)
+Module Ltac2Magic.
+  Import Ltac2 Constr.
+
+  Ltac2 reveal_fixpoint fn :=
+    match Unsafe.kind fn with
+    | Unsafe.Constant cst _ =>
+      Std.eval_unfold [(Std.ConstRef cst, Std.AllOccurrences)] fn
+    | _ => Control.throw Not_found
+    end.
+
+  Ltac2 unfold_fixpoint_once fn :=
+    let fixpoint := reveal_fixpoint fn in
+    match Unsafe.kind fixpoint with
+    | Unsafe.Fix _ _ binders bodies =>
+      let binder := Array.get binders 0 in
+      let unbound_body := Array.get bodies 0 in
+      let body := Unsafe.substnl [fn] 0 unbound_body in
+      match Unsafe.check body with
+      | Val b => b
+      | Err error => Control.throw error
+      end
+    | _ => Control.throw Not_found
+    end.
+
+  Notation unfold_fixpoint_once fn :=
+    ltac2:(let fn := Constr.pretype fn in
+           let fn := unfold_fixpoint_once fn in exact $fn) (only parsing).
+End Ltac2Magic.
+
+Notation beta x :=
+  ltac:(let x := (eval cbv beta in x) in exact x) (only parsing).
+
+Lemma styp2ttyp_eqn : forall A,
+    styp2ttyp A =
+    beta((Ltac2Magic.unfold_fixpoint_once styp2ttyp) A).
+Proof. intros; destruct A; reflexivity. Qed.
+
+Lemma ttyp_trans_ord_top : forall A,
+    check_toplike A = true -> |[A]| = ttyp_top.
+Proof with simpl; eauto.
+  introv HC.
+  rewrite styp2ttyp_eqn. rewrite* HC.
+Qed.
+
+#[local] Hint Resolve ttyp_trans_ord_top : core.
+
+Lemma foldl_append_singleton_list : forall T,
+    list_string_2_string [T] = T.
+Proof.
+  introv. simpl. eauto.
+Qed.
+
+Lemma check_toplike_sound_complete : forall A,
+    toplike A <-> check_toplike A = true.
+Proof.
+  split; introv HT.
+  - induction HT; simple*.
+    rewrite IHHT1. rewrite* IHHT2.
+  - induction* A.
+    all: simpl in HT; try discriminate.
+    forwards* (?&?): andb_prop_elim (check_toplike A1) (check_toplike A2).
+    eauto with bool.
+    constructor; intuition eauto using Is_true_eq_true.
+Qed.
+
+Lemma stype2string_toplike : forall A,
+    check_toplike A = true -> || A || = nil.
+Proof with eauto.
+  introv HT.
+  destruct A; simpl in HT; try discriminate; simpl...
+  all: rewrite* HT.
+Qed.
+
+Lemma nodup_nil_rev : forall l : list string,
+    nodup string_dec l = nil -> l = nil.
+Proof.
+  introv HE. induction* l.
+  - simpl in HE. case_if*. forwards: IHl HE. subst.
+    inverts C.
+Qed.
+
+Lemma list_app_nil_inv : forall l1 l2 : list string,
+    (l1 ++ l2) %list = nil -> l1 = nil /\ l2 = nil.
+Proof.
+  introv HE. destruct l1; destruct* l2; try discriminate.
+Qed.
+
+Lemma stype2string_toplike_inv : forall A,
+    || A || = nil -> check_toplike A = true.
+Proof with eauto using Permutation_sym.
+  introv HT.
+  induction* A;  simpl in HT; try case_if; try discriminate; simpl...
+  - apply nodup_nil_rev in HT.
+    forwards: Permuted_merge (|| A1 ||) (|| A2 ||). rewrite HT in H.
+    forwards: Permutation_nil (|| A1 || ++ || A2 ||)%list...
+    forwards (?&?): list_app_nil_inv H0.
+    forwards*: IHA1. forwards*: IHA2. rewrite H3. rewrite* H4.
+Qed.
+
+Lemma stype2string_and : forall A B : typ,
+    || typ_and A B || = nodup string_dec (merge (stype2string A) (stype2string B)).
+Proof.
+  introv. simpl.
+  destruct (check_toplike A) eqn:HA. destruct (check_toplike B) eqn:HB.
+  all: try ( rewrite (stype2string_toplike A); [ | eassumption] ).
+  all: try ( rewrite (stype2string_toplike B); [ | eassumption] ).
+  all: autorewrite with merge; simpl; eauto.
+Qed.
+
+Lemma typeindex_sorted: forall A,
+    sorted (|| A ||).
+Proof with eauto.
+  introv. induction* A; simpl...
+  all: unfolds...
+  all: try econstructor...
+  - case_if...
+    econstructor...
+  - case_if... applys* merge_sorted_dedup.
+  - case_if...
+    econstructor...
+Qed.
+
+Lemma NoDup_single : forall (x:string), NoDup [x]. Admitted.
+
+Lemma typeindex_nodup: forall A,
+    NoDup (|| A ||).
+Proof with eauto using NoDup_nil, NoDup_single, NoDup_nodup.
+  introv. destruct* A; simpl; try case_if*...
+Qed.
+
+
+Lemma nodup_empty_inv : forall l,
+    nodup string_dec l = nil -> l = nil.
+Proof.
+  introv HE. induction* l.
+  simpl in HE. case_if.
+  exfalso. forwards~: IHl. subst. inverts C.
+Qed.
+
+Lemma merge_empty_inv : forall l r,
+    merge l r = nil -> l = nil /\ r = nil.
+Proof.
+  introv HE. destruct* l; destruct* r.
+  simpl in HE. case_if.
+Qed.
+
+Lemma stype2string_toplike_complete : forall A,
+    || A || = nil -> toplike A.
+Proof with eauto.
+  introv HT. apply check_toplike_sound_complete.
+  induction A; simpl in HT; try discriminate; try case_if; simpl...
+  apply nodup_empty_inv in HT.
+  forwards (?&?): merge_empty_inv HT.
+  forwards~: IHA1. forwards~: IHA2. rewrite H1. rewrite* H2.
+Qed.
+
+(* refine subtypespec *)
+Inductive subTarget : ttyp -> ttyp -> Prop :=
+ | ST_refl : forall At,
+     subTarget At At
+| ST_arrow : forall At Bt At' Bt',
+    subTarget At At' -> subTarget At' At -> subTarget Bt Bt' -> subTarget Bt' Bt -> subTarget (ttyp_arrow At Bt) (ttyp_arrow At' Bt')
+ | ST_rcd : forall At Bt,
+     (forall l Ct, Tlookup l At = Some Ct -> exists Ct', Tlookup l Bt = Some Ct' /\ subTarget Ct' Ct) ->
+     subTarget Bt At.
+
+#[local] Hint Constructors subTarget : core.
+
+Lemma ST_top: forall A, subTarget |[ A ]| ttyp_top.
+Proof with simpl in *; discriminate.
+  introv. applys ST_rcd.
+  intros...
+Qed.
+
+Lemma ST_trans: forall A B C, subTarget A B -> subTarget B C -> subTarget A C.
+Proof with try simpl in *; discriminate.
+  introv HA HB.
+  indTypSize (size_ttyp A + size_ttyp B + size_ttyp C).
+  destruct* HA; inverts* HB.
+  - applys ST_rcd. intros.
+    forwards (?&?&?): H0 H1. forwards (?&?&?): H H2.
+    forwards: IH H5 H3; elia. eauto.
+Qed.
+
+Lemma ST_inv : forall A B,
+    subTarget |[ A ]| |[ B ]| ->
+    forall l Ct, Tlookup l |[ B ]| = Some Ct -> exists Ct', Tlookup l |[ A ]| = Some Ct' /\ subTarget Ct' Ct.
+Proof.
+  introv HA.  inverts* HA.
+  - introv HL. forwards*: H HL.
+Qed.
+
+Lemma ST_andl : forall A B, subTarget |[ (typ_and A B) ]| |[ A ]|.
+Proof with unify_lookup; intuition eauto.
+  introv. applys* ST_rcd.
+  introv HL. simpl. case_if*. apply andb_prop in C...
+  - forwards: ttyp_trans_ord_top H...
+  - forwards: lookup_concat_simpl HL. rewrite H. rewrite HL...
+Qed.
+
+#[local] Hint Resolve ST_top ST_andl : core.
+
+(* soundness of sub to type index translation function *)
+
+Lemma incl_single: forall (x y : string), incl [x] [y] -> x = y.
+Proof.
+  introv HI.
+  apply incl_Forall_in_iff in HI.
+  apply Forall_inv in HI.
+  apply in_one_iff in HI. eauto.
+Qed.
+
+Lemma incl_eq : forall (l1 l2 : list string), l1 = l2 -> incl l1 l2.
+Proof.
+  introv Heq. rewrite Heq. applys* incl_refl.
+Qed.
+
+Lemma incl_eq_tindex: forall A B,
+    incl (||A||) (||B||) -> incl (||B||) (||A||) -> ||A|| = ||B||.
+Proof with eauto using typeindex_nodup, typeindex_sorted.
+  introv HA HB.
+  forwards: NoDup_Permutation_bis HA...
+  apply NoDup_incl_length in HB...
+  applys sorted_unique...
+Qed.
+
+Lemma incl_nodup_merge : forall A1 A2,
+    incl ((|| A1 ||) ++ (|| A2 ||)) (nodup string_dec (merge (|| A1 ||) (|| A2 ||))).
+Proof.
+  introv. apply nodup_incl.
+  forwards: Permuted_merge (|| A1 ||) (|| A2 ||).
+  applys incl_Forall_in_iff. applys Forall_forall. introv HI.
+  applys Permutation_in H HI.
+Qed.
+
+Theorem nodup_incl2: forall {A: Type} (decA: forall x y: A, {x = y} + {x <> y}) (l1 l2: list A),
+    incl l1 l2 -> incl (nodup decA l1) l2.
+Proof.
+  introv HI. applys incl_tran l1.
+  applys nodup_incl. applys incl_refl. eauto.
+Qed.
+
+Lemma incl_nodup_merge_rev : forall A1 A2,
+    incl (nodup string_dec (merge (|| A1 ||) (|| A2 ||))) ((|| A1 ||) ++ (|| A2 ||)).
+Proof.
+  introv. applys (nodup_incl2 string_dec).
+  forwards: Permuted_merge (|| A1 ||) (|| A2 ||).
+  applys incl_Forall_in_iff. applys Forall_forall. introv HI.
+  apply Permutation_sym in H. applys Permutation_in H HI.
+Qed.
+
+Search (_ ++ _ = _ ++ _). (* better use an inductive type as a label *)
+Lemma st_eq1 : forall A1 B1 A2 B2,
+    || B1 || ++
+        String (Ascii.Ascii true false true true false true false false)
+          (String (Ascii.Ascii false true true true true true false false) (|| B2 || ++ ")")) =
+        || A1 || ++
+        String (Ascii.Ascii true false true true false true false false)
+        (String (Ascii.Ascii false true true true true true false false) (|| A2 || ++ ")"))
+    -> || B1 || = || A1 ||.
+Admitted.
+
+Lemma st_eq2 : forall A1 B1 A2 B2,
+      || B1 || ++
+        String (Ascii.Ascii true false true true false true false false)
+          (String (Ascii.Ascii false true true true true true false false) (|| B2 || ++ ")")) =
+        || A1 || ++
+        String (Ascii.Ascii true false true true false true false false)
+        (String (Ascii.Ascii false true true true true true false false) (|| A2 || ++ ")"))
+      -> || B2 || = || A2 ||.
+Admitted.
+Lemma st_eq3 : forall A B l l0,
+ l ++
+        String (Ascii.Ascii true false true true true true false false)
+          (String (Ascii.Ascii false true true true true true false false) (|| B || ++ "}")) =
+        l0 ++
+        String (Ascii.Ascii true false true true true true false false)
+        (String (Ascii.Ascii false true true true true true false false) (|| A || ++ "}"))
+        -> || B || = || A ||.
+Admitted.
+Lemma st_eq4: forall A B l l0,
+ l ++
+        String (Ascii.Ascii true false true true true true false false)
+          (String (Ascii.Ascii false true true true true true false false) (|| B || ++ "}")) =
+        l0 ++
+        String (Ascii.Ascii true false true true true true false false)
+        (String (Ascii.Ascii false true true true true true false false) (|| A || ++ "}"))
+        -> l = l0.
+Admitted.
+
+Lemma eqIndTyp_complete_alt_gen : forall A B,
+    incl (|| B ||) (|| A ||) -> sub A B.
+Proof with eauto using NoDup_nodup, merge_sorted_dedup, check_toplike_sound_complete.
+  (* introv HE. indTypSize (size_typ A + size_typ B). *)
+  (* destruct A; intros. *)
+  (* - forwards*: stype2string_toplike_complete B... simpl in HE. *)
+  (*   applys* incl_l_nil. *)
+  (* - (* bot sub all *) eauto. admit. *)
+  (* - simpl in HE. Search incl. destruct B... *)
+  (*   all: try solve [simpl in HE; try case_if; forwards: incl_single HE; try discriminate]. *)
+  (*   + simpl in HE. case_if. admit. *)
+  (*     forwards: incl_single HE. discriminate. *)
+  (*   + admit. *)
+  (*   + admit. *)
+  (* - (* arrow *) *)
+  (*   simpl in HE. case_if. *)
+  (*   + admit. *)
+  (*     (* stype2string_toplike_complete *) *)
+  (*   + destruct B... *)
+  (*     all: try solve [simpl in HE; try case_if; try discriminate]. *)
+  (*     3: { *)
+  (*       (* arrow *) *)
+  (*       simpl in HE. case_if. admit. *)
+  (*       forwards: incl_single HE. *)
+  (*       injection H. intro HEq. *)
+  (*       Search (_ ++ _ = _ ++ _). (* better use an inductive type as a label *) *)
+  (*       assert (|| B1 || = || A1 ||) by admit. assert (|| A2 || = || B2 ||) by admit. *)
+  (*       assert (|| A1 || = || B1 ||) by admit. assert (|| B2 || = || A2 ||) by admit. *)
+  (*       forwards: IH B1 A1; eauto using incl_eq. elia. *)
+  (*       forwards: IH A1 B1; eauto using incl_eq. elia. *)
+  (*       forwards: IH A2 B2; eauto using incl_eq. elia. *)
+  (*       forwards: IH B2 A2; eauto using incl_eq. elia. *)
+  (*     } *)
+  (*     3: { (* and *) admit. *)
+  (*          (* forwards ([|]&[|]): stype2string_single_and_inv HE. *) *)
+  (*          (* simpl in HE. rewrite <- H0 in HE. *) *)
+  (*          (* case_if in HE. *) *)
+  (*          (* assert (Heq: nodup string_dec (syntax_ott.NSort.merge nil (|| B2 ||)) = || B2 ||) by admit. *) *)
+  (*          (* rewrite Heq in HE. forwards: IHB2 HE. elia. *) *)
+  (*          (* forwards*: stype2string_toplike_complete B1. *) *)
+  (*     } *)
+  (*     admit. admit. admit. *)
+  (* - simpl in HE. case_if. admit. *)
+  (*   assert (incl (nodup string_dec (syntax_ott.NSort.merge (|| A1 ||) (|| A2 ||))) ((|| A1 ||) ++ (|| A2 ||))). { *)
+  (*     applys nodup_incl string_dec. *)
+  (*     Search (incl). admit. *)
+  (*   } *)
+  (*   forwards: incl_tran HE H. *)
+  (* (*   + admit. (* top *) *) *)
+  (* (*   + admit. (* single *) *) *)
+  (* (*   + admit. (* single *) *) *)
+  (* (*   + admit. (* single *) *) *)
+  (* (*   + (* prove (typ_and A1 A2) <: B1 *) *) *)
+  (* (*     (* prove (typ_and A1 A2) <: B2 *) *) *)
+  (* (*     assert (incl (|| A1 ||) (|| typ_and A1 A2 ||)). *) *)
+  (* (*     assert (incl (|| A2 ||) (|| typ_and A1 A2 ||)). *) *)
+  (* (*     all: admit. *) *)
+  (* (*   + admit. (* single *) *) *)
+  (* (* - admit. *) *)
+  (*   Restart. *)
+  Proof with eauto using incl_tran, incl_appl, incl_appr, incl_nil.
+  introv HE. indTypSize (size_typ A + size_typ B).
+  destruct B; intros; eauto.
+  - simpl in HE.
+    apply incl_Forall_in_iff in HE.
+    apply Forall_inv in HE.
+    destruct A; simpl in HE; try solve [try case_if; try destruct HE; try discriminate; intuition eauto; inverts H].
+    + case_if.
+      forwards Hia: In_incl HE incl_nodup_merge_rev.
+      forwards [|]: in_app_or Hia.
+      * assert (incl (||typ_bot||) (||A1||)). {
+         simpl. unfolds. intros. rewrite in_one_iff in H0. subst*.
+        }
+        forwards*: IH H0. elia.
+      * assert (incl (||typ_bot||) (||A2||)). {
+         simpl. unfolds. intros. rewrite in_one_iff in H0. subst*.
+        }
+        forwards*: IH H0. elia.
+  - simpl in HE.
+    apply incl_Forall_in_iff in HE.
+    apply Forall_inv in HE.
+    destruct A; simpl in HE; try solve [try case_if; try destruct HE; try discriminate; intuition eauto; inverts H].
+    + case_if.
+      forwards Hia: In_incl HE incl_nodup_merge_rev.
+      forwards [|]: in_app_or Hia.
+      * assert (incl (||typ_base||) (||A1||)). {
+         simpl. unfolds. intros. rewrite in_one_iff in H0. subst*.
+        }
+        forwards*: IH H0. elia.
+      * assert (incl (||typ_base||) (||A2||)). {
+         simpl. unfolds. intros. rewrite in_one_iff in H0. subst*.
+        }
+        forwards*: IH H0. elia.
+  - simpl in HE; try case_if.
+    { rewrite <- check_toplike_sound_complete in C... }
+    try apply incl_Forall_in_iff in HE.
+    try apply Forall_inv in HE.
+    destruct A; simpl in HE; try solve [try case_if; try destruct HE; try discriminate; intuition eauto; inverts H].
+    + (* arrow vs arrow *)
+      simpl in HE. case_if.
+      rewrite in_one_iff in HE.
+      injection HE. intro HEq.
+      assert (|| B1 || = || A1 ||) by eauto using st_eq1.
+      assert (|| A2 || = || B2 ||) by eauto using st_eq2.
+      assert (|| A1 || = || B1 ||) by eauto using st_eq1.
+      assert (|| B2 || = || A2 ||) by eauto using st_eq2.
+      forwards: IH B1 A1; eauto using incl_eq. elia.
+      forwards: IH A1 B1; eauto using incl_eq. elia.
+      forwards: IH A2 B2; eauto using incl_eq. elia.
+      forwards: IH B2 A2; eauto using incl_eq. elia.
+    + case_if.
+      forwards Hia: In_incl HE incl_nodup_merge_rev.
+      forwards [|]: in_app_or Hia.
+      * assert (incl (||typ_arrow B1 B2||) (||A1||)). {
+         simpl. unfolds. intros. case_if. rewrite in_one_iff in H0. subst*.
+        }
+        forwards*: IH H0. elia.
+      * assert (incl (||typ_arrow B1 B2||) (||A2||)). {
+         simpl. unfolds. intros. case_if. rewrite in_one_iff in H0. subst*.
+        }
+        forwards*: IH H0. elia.
+  - assert (incl (|| B1 ||)(|| typ_and B1 B2 ||)). {
+      simpl. case_if. { forwards (?&?): andb_prop C. rewrite* stype2string_toplike. eauto...  }
+      applys incl_tran. 2: applys incl_nodup_merge. applys incl_appl. applys incl_refl.
+    }
+    assert (incl (|| B2 ||)(|| typ_and B1 B2 ||)). {
+      simpl. case_if. { forwards (?&?): andb_prop C. rewrite* stype2string_toplike. eauto...  }
+      applys incl_tran. 2: applys incl_nodup_merge. applys incl_appr. applys incl_refl.
+    }
+    forwards: incl_tran H HE. forwards: incl_tran H0 HE.
+    forwards*: IH A B1. elia. forwards*: IH A B2. elia.
+  - simpl in HE; try case_if.
+    { rewrite <- check_toplike_sound_complete in C... }
+    try apply incl_Forall_in_iff in HE.
+    try apply Forall_inv in HE.
+    destruct A; simpl in HE; try solve [try case_if; try destruct HE; try discriminate; intuition eauto; inverts H].
+    + case_if.
+      forwards Hia: In_incl HE incl_nodup_merge_rev.
+      forwards [|]: in_app_or Hia.
+      * assert (incl (||typ_rcd l B||) (||A1||)). {
+         simpl. unfolds. intros. case_if. rewrite in_one_iff in H0. subst*.
+        }
+        forwards*: IH H0. elia.
+      * assert (incl (||typ_rcd l B||) (||A2||)). {
+         simpl. unfolds. intros. case_if. rewrite in_one_iff in H0. subst*.
+        }
+        forwards*: IH H0. elia.
+    + simpl in HE. case_if.
+      rewrite in_one_iff in HE.
+      injection HE. intro HEq.
+      assert (|| B || = || A ||) by eauto using st_eq3. assert (|| A || = || B ||) by eauto using st_eq3.
+      assert (l = l0) by eauto using st_eq4. subst.
+      forwards: IH B A; eauto using incl_eq. elia.
+      forwards*: IH A B; eauto using incl_eq. elia.
+  Qed.
+
+Corollary eqIndTyp_complete : forall A B,
+    (|| A ||) = (|| B ||) -> sub A B /\ sub B A.
+Proof with eauto using incl_refl.
+  introv HE.
+  split; applys eqIndTyp_complete_alt_gen.
+  rewrite HE... rewrite <- HE...
+Qed.
+
+Lemma eqIndTyp_sound_alt_gen : forall A B,
+    sub A B -> incl (|| B ||) (|| A ||).
+Proof with eauto using incl_nil, incl_nodup_merge, NoDup_nodup, merge_sorted_dedup, check_toplike_sound_complete.
+  introv HS.
+  induction HS; try solve [simpl; eauto using incl_refl].
+  - rewrite check_toplike_sound_complete in H. rewrite* stype2string_toplike...
+  - simpl. case_if. applys incl_nil.
+    case_if. {
+      forwards*: stype2string_toplike A2...
+      forwards*: incl_eq_tindex A2 B2. rewrite H0 in H.
+      forwards*: stype2string_toplike_inv H. rewrite H1 in C. discriminate.
+    }
+    applys incl_eq.
+    forwards*: incl_eq_tindex A1 B1. forwards*: incl_eq_tindex A2 B2.
+    rewrite H. rewrite H0...
+  - simpl. case_if. applys incl_nil.
+    case_if. {
+      forwards*: stype2string_toplike A...
+      forwards*: incl_eq_tindex A B. rewrite H0 in H.
+      forwards*: stype2string_toplike_inv H. rewrite H1 in C. discriminate.
+    }
+    applys incl_eq.
+    forwards*: incl_eq_tindex A B.
+    rewrite* H.
+  - applys incl_tran IHHS.
+    simpl. case_if.
+    { forwards* (?&?): andb_prop C. rewrite* stype2string_toplike...  }
+    applys incl_tran incl_nodup_merge...
+    applys incl_appl. applys incl_refl.
+  - applys incl_tran IHHS.
+    simpl. case_if.
+    { forwards* (?&?): andb_prop C. rewrite* stype2string_toplike...  }
+    applys incl_tran incl_nodup_merge...
+    applys incl_appr. applys incl_refl.
+  - simpl. case_if. applys incl_nil.
+    applys incl_tran incl_nodup_merge_rev.
+    applys* incl_app.
+Qed.
+
+Corollary eqIndTyp_sound_alt : forall B A,
+    sub B A -> sub A B -> (|| B ||) = (|| A ||).
+Proof.
+  introv HS1 HS2.
+  apply eqIndTyp_sound_alt_gen in HS1.
+  apply eqIndTyp_sound_alt_gen in HS2.
+  applys* incl_eq_tindex.
+Qed.
+
+(* sub target for eq index target *)
+Lemma lookup_eq : forall A B,
+    subTarget A B -> subTarget B A -> forall l, Tlookup l A = None -> Tlookup l B = None.
+Proof.
+  introv HS HR.
+  induction* HS.
+  - introv HL. remember (Tlookup l At). destruct* o.
+    forwards* (?&?&?): H l. rewrite HL in H0. discriminate.
+Qed.
+
+Lemma sub_eqv_toplike : forall A B,
+    sub B A -> sub A B -> check_toplike B = check_toplike A.
+Proof with try rewrite* <- check_toplike_sound_complete.
+  introv HA HB. induction* HA.
+  - apply check_toplike_sound_complete in H. rewrite H.
+    apply check_toplike_sound_complete in H. apply check_toplike_sound_complete.
+    inductions HB; try solve [inverts~ H]...
+  - admit. - admit. - admit.
+Admitted.
+
+Lemma Tlookup_eq : forall l l' A B,
+    Tlookup l (ttyp_rcd l' A ttyp_top) = Some B -> l = l' /\ A = B.
+Admitted.
+
+Lemma sub_source2target_aux : forall A B l T T',
+    (Tlookup l (|[ A ]|) = Some T -> Tlookup l (|[ B ]|) = Some T' -> subTarget T T') /\
+    (sub A B -> subTarget |[A]| |[B]|).
+Proof with try rewrite* <- check_toplike_sound_complete; simpl in *; try case_if; try discriminate; eauto.
+  introv. gen l. indTypSize (size_typ A + size_typ B).
+  split.
+  { destruct A; introv HA HB. 1-3: clear IH.
+  - rewrite* (ttyp_trans_ord_top) in HA...
+  - simpl in HA. case_if. inverts HA. rewrite C in HB.
+    induction B...
+    + inverts HB...
+    + destruct_lookup HB. forwards*: IHB1. elia. forwards*: IHB2. elia.
+  - (* base *) simpl in HA. case_if. inverts HA. rewrite C in HB.
+    induction B...
+    + inverts HB...
+    + destruct_lookup HB. forwards*: IHB1. elia. forwards*: IHB2. elia.
+  - (* arrow *) simpl in HA. case_if. inverts HA. case_if.
+    rewrite C0 in HB.
+    induction B...
+    + forwards (?&?): Tlookup_eq HB. inverts H0. rewrite <- H1.
+      inverts H.
+      assert (HE1: || A1 || = || B1 ||) by eauto using st_eq1.
+      assert (HE2: || A2 || = || B2 ||) by eauto using st_eq2.
+      (* assert (HS: forall A B, sub A B -> subTarget |[A]| |[B]|) by admit. *)
+      forwards (HS1&HS2): eqIndTyp_complete HE1. forwards (HS3&HS4): eqIndTyp_complete HE2.
+      forwards~ (_&HS1'): IH A1 B1. elia. forwards~: HS1'.
+      forwards~ (_&HS2'): IH B1 A1. elia. forwards~: HS2'.
+      forwards~ (_&HS3'): IH A2 B2. elia. forwards~: HS3'.
+      forwards~ (_&HS4'): IH B2 A2. elia.
+    + destruct_lookup HB. forwards*: IHB1. elia. forwards*: IHB2. elia.
+  - (* and *) simpl in HA. case_if. destruct_lookup HA.
+    + forwards* (?&_): IH A1 B. elia. + forwards* (?&_): IH A2 B. elia.
+  - (* rcd *) simpl in HA. case_if. inverts HA. case_if.
+    rewrite C0 in HB.
+    induction B...
+    + destruct_lookup HB. forwards*: IHB1. elia. forwards*: IHB2. elia.
+    + forwards (?&?): Tlookup_eq HB. inverts H0. rewrite <- H1.
+      inverts H.
+      assert (HE1: || A || = || B ||) by eauto using st_eq3.
+      (* assert (HS: forall A B, sub A B -> subTarget |[A]| |[B]|) by admit. *)
+      forwards (HS1&HS2): eqIndTyp_complete HE1.
+      forwards* (_&HS1'): IH A B. elia.
+  }
+
+  { introv HS.
+    destruct HS. all: try solve [simpl; eauto].
+    - rewrite* (ttyp_trans_ord_top B)...
+    - simpl. case_if*; simpl; case_if*.
+      { forwards* HSE: sub_eqv_toplike B2 A2. rewrite C0 in HSE. rewrite C in HSE. discriminate. }
+      { forwards* HSE: sub_eqv_toplike B2 A2. rewrite C0 in HSE. rewrite C in HSE. discriminate. }
+      +
+        rewrite* (eqIndTyp_sound_alt A1 B1). rewrite* (eqIndTyp_sound_alt A2 B2).
+        applys ST_rcd. introv HL. simpl in HL. case_if*.
+        subst. exists. split*. injection HL. intro HE. subst*.
+    - simpl. case_if*; simpl; case_if*.
+      { forwards* HSE: sub_eqv_toplike B A. rewrite C0 in HSE. rewrite C in HSE. discriminate. }
+      { forwards* HSE: sub_eqv_toplike B A. rewrite C0 in HSE. rewrite C in HSE. discriminate. }
+      +
+        rewrite* (eqIndTyp_sound_alt A B).
+        applys ST_rcd. introv HL. simpl in HL. case_if*.
+        subst. exists. split*. injection HL. intro HE. subst*.
+        forwards* (_&?): IH A B. elia.
+    - forwards* (_&?): IH A1 A3. elia. applys* ST_trans.
+    - forwards* (_&IHHS'): IH A2 A3. elia. forwards~ IHHS: IHHS'.
+      applys* ST_trans IHHS. clear HS.
+      { applys* ST_rcd.
+        introv HL. simpl. case_if*. apply andb_prop in C; unify_lookup; intuition eauto.
+        - forwards: ttyp_trans_ord_top H0; unify_lookup; intuition eauto.
+        - remember (check_toplike A1). destruct b.
+          + forwards*: ttyp_trans_ord_top A1; unify_lookup; intuition eauto.
+            rewrite H. simpl; unify_lookup; intuition eauto.
+          + remember (Tlookup l0 |[A1]|). destruct o.
+            * forwards*: lookup_concat_simpl (|[ A1 ]|) (|[ A2 ]|). rewrite H.
+              rewrite <- Heqo; unify_lookup. exists t. split.
+              now eauto.
+              forwards (IH1&_): IH A1 A2. elia. applys* IH1.
+            * forwards*: lookup_concat_simpl_none (|[ A1 ]|) (|[ A2 ]|). rewrite H.
+              rewrite* HL.
+      }
+    - simpl. case_if*.
+      forwards* (_&IHHS1'): IH A1 A2. elia. forwards~ IHHS1: IHHS1'.
+      forwards* (_&IHHS2'): IH A1 A3. elia. forwards~ IHHS2: IHHS2'.
+    + applys ST_rcd. introv HL.
+      destruct_lookup HL.
+      * forwards* (?&?&?): ST_inv IHHS1.
+      * forwards* (?&?&?): ST_inv IHHS2.
+  }
+  Unshelve. all: econstructor.
+Qed.
+
+Lemma lookup_sub : forall A B l T T',
+  Tlookup l (|[ A ]|) = Some T -> Tlookup l (|[ B ]|) = Some T' -> subTarget T T'.
+Proof.
+  introv. forwards (?&_): sub_source2target_aux. applys H.
+Qed.
+
+Lemma sub_source2target : forall A B,
+    sub A B -> subTarget |[A]| |[B]|.
+Proof.
+  introv. forwards (_&?): sub_source2target_aux. applys H.
+  Unshelve. all: econstructor.
+Qed.
+
+Search sub.
+
+(* Lemma lookup_sub : forall A B l T T', *)
+(*     Tlookup l (|[ A ]|) = Some T  -> *)
+(*     Tlookup l (|[ B ]|) = Some T' -> subTarget T T'. *)
+(* Proof with simpl in *; try case_if; try discriminate; eauto. *)
+(*   introv HA HB. *)
+(*   induction A. *)
+(*   - rewrite* (ttyp_trans_ord_top) in HA... *)
+(*   - simpl in HA. case_if. inverts HA. rewrite C in HB. *)
+(*     induction B... *)
+(*     + inverts HB... *)
+(*     + destruct_lookup HB. forwards*: IHB1. forwards*: IHB2. *)
+(*   - simpl in HA. case_if. inverts HA. rewrite C in HB. *)
+(*     induction B... *)
+(*     + inverts HB... *)
+(*     + destruct_lookup HB. forwards*: IHB1. forwards*: IHB2. *)
+(*   - clear IHA1 IHA2. simpl in HA. case_if. inverts HA. case_if. *)
+(*     rewrite C0 in HB. *)
+(*     induction B... *)
+(*     + forwards (?&?): Tlookup_eq HB. inverts H0. rewrite <- H1. *)
+(*       assert (HE1: || A1 || = || B1 ||) by admit. assert (HE2: || A2 || = || B2 ||) by admit. *)
+(*       assert (HS: forall A B, sub A B -> subTarget |[A]| |[B]|) by admit. *)
+(*       forwards (HS1&HS2): eqIndTyp_complete HE1. forwards (HS3&HS4): eqIndTyp_complete HE2. *)
+(*       apply HS in HS1. apply HS in HS2. apply HS in HS3. apply HS in HS4... *)
+(*     + destruct_lookup HB. forwards*: IHB1. forwards*: IHB2. *)
+(*   - simpl in HA. case_if. destruct_lookup HA. *)
+(*     + forwards~: IHA1. + forwards~: IHA2. *)
+(*   - clear IHA. simpl in HA. case_if. inverts HA. case_if. *)
+(*     rewrite C0 in HB. *)
+(*     induction B... *)
+(*     + destruct_lookup HB. forwards*: IHB1. forwards*: IHB2. *)
+(*     + forwards (?&?): Tlookup_eq HB. inverts H0. rewrite <- H1. *)
+(*       assert (HE1: || A || = || B ||) by admit. *)
+(*       assert (HS: forall A B, sub A B -> subTarget |[A]| |[B]|) by admit. *)
+(*       forwards (HS1&HS2): eqIndTyp_complete HE1. *)
+(*       apply HS in HS1. apply HS in HS2... *)
+(* Admitted. *)
+
+(* (* Lemma lookup_sub : forall A B l T, *) *)
+(* (*     sub A B -> *) *)
+(* (*     Tlookup l (|[ B ]|) = Some T -> *) *)
+(* (*     exists T', Tlookup l (|[ A ]|) = Some T' /\ subTarget T T'. *) *)
+(* (* Proof with try rewrite* <- check_toplike_sound_complete. *) *)
+(* (*   introv HS HL. *) *)
+(* (*   induction HS; try solve [simpl; eauto]. *) *)
+(* (*   - rewrite* (ttyp_trans_ord_top B) in HL... inverts HL. *) *)
+(* (*   - simpl in HL. case_if. inverts HL. case_if. *) *)
+(* (*     injection H0. intro HE. rewrite C0. *) *)
+(* (*     exists*. split. simpl. case_if. *) *)
+(* (*     { forwards* HSE: sub_eqv_toplike B2 A2. rewrite C1 in HSE. rewrite C in HSE. *) *)
+(* (*       discriminate. } *) *)
+(* (*     forwards*: eqIndTyp_sound_alt B1 A1. forwards*: eqIndTyp_sound_alt B2 A2. *) *)
+(* (*     rewrite H. rewrite* H1. *) *)
+(* (*     rewrite* <- HE. *) *)
+(* (*   - simpl in HL. case_if. inverts HL. case_if. *) *)
+(* (*     injection H0. intro HE. rewrite C0. *) *)
+(* (*     exists*. split. simpl. case_if. *) *)
+(* (*     { forwards* HSE: sub_eqv_toplike B A. rewrite C1 in HSE. rewrite C in HSE. *) *)
+(* (*       discriminate. } *) *)
+(* (*     forwards*: eqIndTyp_sound_alt B A. *) *)
+(* (*     rewrite H. rewrite* <- HE. rewrite* <- HE. *) *)
+(* (*     admit. *) *)
+(* (*   - *) *)
+
+(* (* REQUIRES ST_ANDR *) *)
+(* Lemma sub_source2target : forall A B, *)
+(*     sub A B -> subTarget |[A]| |[B]|. *)
+(* Proof with try rewrite* <- check_toplike_sound_complete. *)
+(*   introv HS. *)
+(*   induction HS; try solve [simpl; eauto]. *)
+(*   - rewrite* (ttyp_trans_ord_top B)... *)
+(*   - simpl. case_if*. admit. *)
+(*     simpl. case_if*. admit. *)
+(*     + *)
+(*       rewrite* (eqIndTyp_sound_alt A1 B1). rewrite* (eqIndTyp_sound_alt A2 B2). *)
+(*       applys ST_rcd. introv HL. simpl in HL. case_if*. *)
+(*       subst. exists. split*. injection HL. intro HE. subst*. *)
+(*   - simpl. case_if*. admit. *)
+(*     simpl. case_if*. admit. *)
+(*     + *)
+(*       rewrite* (eqIndTyp_sound_alt A B). *)
+(*       applys ST_rcd. introv HL. simpl in HL. case_if*. *)
+(*       subst. exists. split*. injection HL. intro HE. subst*. *)
+(*   - applys* ST_trans IHHS. *)
+(*   - applys* ST_trans IHHS. clear HS. *)
+(*     { applys* ST_rcd. *)
+(*       introv HL. simpl. case_if*. apply andb_prop in C; unify_lookup; intuition eauto. *)
+(*       - forwards: ttyp_trans_ord_top H0; unify_lookup; intuition eauto. *)
+(*       - remember (check_toplike A1). destruct b. *)
+(*         + forwards*: ttyp_trans_ord_top A1; unify_lookup; intuition eauto. *)
+(*           rewrite H. simpl; unify_lookup; intuition eauto. *)
+(*         + remember (Tlookup l |[A1]|). destruct o. *)
+(*           * forwards*: lookup_concat_simpl (|[ A1 ]|) (|[ A2 ]|). rewrite H. *)
+(*             rewrite <- Heqo; unify_lookup; intuition eauto. exists*. split*. *)
+(*             applys* lookup_sub. (* !!! *) *)
+(*           * forwards*: lookup_concat_simpl_none (|[ A1 ]|) (|[ A2 ]|). rewrite H. *)
+(*             rewrite* HL. *)
+(*     } *)
+(*   - simpl. case_if*. *)
+(*     + applys ST_rcd. introv HL. *)
+(*       remember (Tlookup l |[A2]|). destruct o. *)
+(*       * forwards* (?&?&?): ST_inv IHHS1. *)
+(*         forwards* : lookup_concat_simpl (|[ A2 ]|) (|[ A3 ]|). *)
+(*         rewrite HL in H1. rewrite <- Heqo in H1. injection H1. intro Heq. subst*. *)
+(*       * forwards* (?&?&?): ST_inv IHHS2. *)
+(*         forwards* : lookup_concat_simpl_none (|[ A2 ]|) (|[ A3 ]|). *)
+(*         rewrite* HL in H. *)
+(* Admitted. *)
+
+
+Lemma ST_andr : forall A B, subTarget |[ (typ_and A B) ]| |[ B ]|.
+Proof with unify_lookup; intuition eauto.
+  introv. applys* ST_rcd.
+  introv HL. simpl. case_if*. apply andb_prop in C...
+  - forwards: ttyp_trans_ord_top H0...
+  - remember (check_toplike A). destruct b.
+    + forwards*: ttyp_trans_ord_top A... rewrite H. simpl...
+    + remember (Tlookup l |[A]|). destruct o.
+      * forwards*: lookup_concat_simpl (|[ A ]|) (|[ B ]|). rewrite H.
+        rewrite <- Heqo... exists*. split*.
+        applys* lookup_sub.
+      * forwards*: lookup_concat_simpl_none (|[ A ]|) (|[ B ]|). rewrite H.
+        rewrite* HL.
+Qed.
+
+(* Main properties on translation are as above *)
 
 Lemma wf_rcd_lookup : forall i T Ti,
   wf_typ T ->
@@ -403,38 +1327,6 @@ Qed.
 (*   - applys IHHE. *)
 (* Admitted. *)
 
-Lemma lookup_concat_simpl : forall i A B T,
-    Tlookup i A = Some T ->
-    Tlookup i (ttyp_concat_simpl A B) = Tlookup i A.
-Proof.
-  introv LK. gen i T B.
-  induction A; intros; simpl in LK; inverts LK.
-  case_if*.
-  - inverts* H0.
-    subst. simpl. case_if*.
-  - simpl. case_if*.
-Qed.
-
-
-Lemma lookup_concat_simpl_none : forall i A B,
-    Tlookup i A = None -> rec_typ A ->
-    Tlookup i (ttyp_concat_simpl A B) = Tlookup i B.
-Proof.
-  introv LK HR. gen i B.
-  induction A; intros; simpl; try solve_by_invert; eauto.
-  - inverts* HR. inverts LK. case_if.
-    forwards* Heq: IHA2.
-Qed.
-
-Lemma rcd_typ_concat_simpl : forall T1 T2,
-    rec_typ T1 -> rec_typ T2 ->
-    rec_typ (ttyp_concat_simpl T1 T2).
-Proof with eauto.
-  introv WF1 WF2.
-  induction WF1...
-  - simpl...
-Qed.
-
 Lemma eqIndTypTarget_concat_comm : forall A B,
     rec_typ A -> rec_typ B ->
     eqIndTypTarget (ttyp_concat_simpl A B) (ttyp_concat_simpl B A).
@@ -485,11 +1377,6 @@ Notation "[[ A ]]" := (styp2ttyp_raw A) (at level 5, A at next level).
 (*   Unshelve. all: econstructor. *)
 (* Qed. *)
 
-Lemma translate_to_record_types : forall A,
-    rec_typ |[ A ]|.
-Proof with eauto using rcd_typ_concat_simpl.
-  introv. induction A; simpl; try case_if; simpl...
-Qed.
 
 Lemma ttyp_trans_wf : forall A,
     wf_typ |[A]|.
@@ -683,31 +1570,6 @@ Admitted.
 
 (* originally in source5 *)
 
-(* Properties on merge *)
-Locate merge.
-Module Import NSort := Sort NTTLB.
-Lemma merge_empty : forall l,
-    merge nil l = l.
-Proof.
-  introv. induction* l.
-Qed.
-
-Lemma merge_empty_r : forall l,
-    merge l nil = l.
-Proof.
-  introv. induction* l.
-Qed.
-
-#[local] Hint Rewrite merge_empty merge_empty_r : merge.
-
-Lemma merge_cons : forall a l b r,
-    merge (a::l) (b::r) =
-      if if proj1_sig (string_compare_lex a b) is Gt then false else true then a :: merge l (b::r) else b :: merge (a::l) r.
-Proof with eauto.
-  introv. induction* l; destruct (proj1_sig (string_compare_lex a b)); autorewrite with merge...
-Qed.
-
-#[local] Hint Rewrite merge_cons : merge.
 
 
 (** * Multisets *)
@@ -833,37 +1695,6 @@ Check NTTLB.leb_trans.
 
 (* no duplication sorted *)
 
-Definition sorted := Sorted lex_lt.
-
-Theorem sorted_unique : forall (l1 l2 : list string),
-    sorted l1 -> sorted l2 -> Permutation l1 l2 -> l1 = l2.
-Proof.
-  introv HS1 HS2 HP.
-  applys* Sort_In_eq lex_lt.
-  applys lex_lt_trans.
-  applys lex_lt_not_eq.
-  split; introv HI;
-    eauto using Permutation_sym, Permutation_in.
-Qed.
-
-Theorem merge_comm : forall (l1 l2 : list string),
-    sorted l1 -> sorted l2 ->
-    merge l1 l2 = merge l2 l1.
-    (* nodup string_dec (merge l1 l2) = nodup string_dec (merge l2 l1). *)
-Proof.
-  introv HS1 HS2.
-  applys* Sort_In_eq lex_lt.
-  admit.
-  applys lex_lt_not_eq.
-  admit. admit.
-  admit.
-  (* - lets HP: Permuted_merge. *)
-  (*   split; introv HI; applys nodup_In; apply nodup_In in HI; *)
-  (*     applys Permutation_in HP. *)
-  (*   all: applys in_app_iff; applys or_comm; applys in_app_iff. *)
-  (*   all: applys Permutation_in HI; applys* Permutation_sym HP. *)
-Admitted.
-
 (* Search Sorted. *)
 (* Admitted. *)
 (*   Search Permutation. *)
@@ -894,22 +1725,6 @@ Admitted.
 (*            eapply eq_equivalence. eapply lex_lt_strorder. *)
 (*            eapply NOTF.lt_compat. *)
 
-Lemma HdRel_nodup : forall a l,
-    Sorted NOTF.le l -> HdRel lex_lt a l -> HdRel lex_lt a (nodup string_dec l).
-Proof with eauto.
-  introv HS HR.
-  applys In_InfA. introv HI. apply nodup_In in HI.
-  induction l.
-  - inverts HI.
-  - apply in_inv in HI. destruct HI.
-    + subst*. inverts* HR.
-    + inverts HS. inverts HR.
-      forwards*: IHl.
-      inverts* H3. constructor.
-      destruct H0. now applys* lex_lt_trans.
-      now subst*.
-Qed.
-
 Lemma le_trans : forall s0 s1 s2 : string, NOTF.le s0 s1 -> NOTF.le s1 s2 -> NOTF.le s0 s2.
 Admitted.
 
@@ -931,20 +1746,6 @@ Lemma sorted_nodup_aux : forall l,
     sorted (nodup string_dec l) -> Sorted NOTF.le l.
 Abort. (* incorrect *)
 
-Lemma sorted_nodup : forall l,
-    Sorted NOTF.le l -> sorted (nodup string_dec l).
-Proof with eauto.
-  introv HS. induction* l.
-  - simpl... econstructor...
-  - inverts HS. forwards*: IHl.
-    simpl. case_if.
-    + apply H.
-    + econstructor... destruct l...
-      * simpl...
-      * applys* HdRel_nodup.
-        inverts H2. inverts* H3.
-        exfalso. applys C. applys in_eq.
-Qed.
 
 (* Lemma HdRel_nodup : forall a l, *)
 (*         HdRel NOTF.le a l -> In b l -> lex_lt a b. *)
@@ -976,55 +1777,6 @@ Qed.
 
 (*       Search (Sorted). *)
 
-Lemma HdRel_relax : forall a l,
-    HdRel lex_lt a l -> HdRel NOTF.le a l.
-Proof with eauto.
-  introv HS. induction* HS. constructor...
-  left*.
-Qed.
-
-Lemma sorted_relax : forall l,
-    sorted l -> Sorted NOTF.le l.
-Proof with eauto.
-  introv HS. induction* HS.
-  destruct H... constructor... constructor...
-  left*.
-Qed.
-
-#[local] Hint Constructors Sorted HdRel : core.
-#[local] Hint Resolve HdRel_relax sorted_relax : core.
-
-Lemma test : forall a l r,
-    HdRel NOTF.le a l -> HdRel NOTF.le a r -> HdRel NOTF.le a (merge l r).
-Admitted.
-
-Lemma merge_sorted : forall l r,
-    sorted l -> sorted r -> Sorted NOTF.le (merge l r).
-Proof with eauto using sorted_relax.
-  introv HSl HSr. gen r.
-  induction HSl; intros; autorewrite with merge...
-  - induction HSr...
-    + autorewrite with merge.
-      constructor...
-    + destruct (string_compare_lex a a0) eqn:HE. destruct c.
-      * subst*. simpl. rewrite HE. simpl...
-        econstructor. applys IHHSl...
-        econstructor... applys test...
-        econstructor... right*.
-      * simpl. rewrite HE. simpl...
-        forwards* IH: IHHSl (a0 :: l0)...
-        all: econstructor...
-        applys test...
-      * simpl. rewrite HE. simpl...
-        econstructor... applys test (a :: l) l0...
-Qed.
-
-Lemma merge_sorted_dedup: forall l r,
-    sorted l -> sorted r -> sorted (nodup string_dec (merge l r)).
-Proof with eauto using sorted_nodup, sorted_relax.
-  introv HSl HSr.
-  forwards: merge_sorted HSl HSr...
-Qed.
 (*   induction HSl; intros; autorewrite with merge... *)
 (*   - induction HSr... *)
 (*     + autorewrite with merge. simpl. case_if... *)
@@ -1097,25 +1849,6 @@ Qed.
 Open Scope string_scope.
 
 (* Properties of type translation *)
-Lemma foldl_append_singleton_list : forall T,
-    list_string_2_string [T] = T.
-Proof.
-  introv. simpl. eauto.
-Qed.
-
-Lemma check_toplike_sound_complete : forall A,
-    toplike A <-> check_toplike A = true.
-Proof.
-  split; introv HT.
-  - induction HT; simple*.
-    rewrite IHHT1. rewrite* IHHT2.
-  - induction* A.
-    all: simpl in HT; try discriminate.
-    forwards* (?&?): andb_prop_elim (check_toplike A1) (check_toplike A2).
-    eauto with bool.
-    constructor; intuition eauto using Is_true_eq_true.
-Qed.
-
 Lemma type2list_arrow : forall A B,
   ~ toplike B ->
   stype2string (typ_arrow A B) = [ ( "(" ++ (stype2string A) ++ "->" ++ (stype2string B) ++ ")" ) ].
@@ -1140,26 +1873,6 @@ Proof.
   right. unfolds. simpl. case_if*.
 Qed.
 
-Lemma stype2string_toplike : forall A,
-    toplike A -> || A || = nil.
-Proof with eauto.
-  introv HT. apply check_toplike_sound_complete in HT.
-  destruct A; simpl in HT; try discriminate; simpl...
-  all: rewrite* HT.
-Qed.
-
-Lemma stype2string_and : forall A B : typ,
-    || typ_and A B || = nodup string_dec (merge (stype2string A) (stype2string B)).
-Proof.
-  introv. simpl.
-  destruct (check_toplike A) eqn:HA. destruct (check_toplike B) eqn:HB.
-  all: try apply check_toplike_sound_complete in HA.
-  all: try apply check_toplike_sound_complete in HB.
-  all: try ( rewrite (stype2string_toplike A); [ | eassumption] ).
-  all: try ( rewrite (stype2string_toplike B); [ | eassumption] ).
-  all: autorewrite with merge; simpl; eauto.
-Qed.
-
 
 Lemma eqIndTyp_toplike : forall A B,
     eqIndTyp A B -> toplike A <-> toplike B.
@@ -1175,24 +1888,7 @@ Qed.
 (*     ||A|| = ||B|| -> type2tlist A = type2tlist B. *)
 (* Proof with intuition eauto. *)
 (*   introv HE. unfold stype2string in HE. rewrite HE. *)
-Lemma typeindex_sorted: forall A,
-    sorted (|| A ||).
-Proof with eauto.
-  introv. induction* A; simpl...
-  all: unfolds...
-  all: try econstructor...
-  - case_if...
-    econstructor...
-  - case_if... applys* merge_sorted_dedup.
-  - case_if...
-    econstructor...
-Qed.
 
-Lemma typeindex_nodup: forall A,
-    NoDup (|| A ||).
-Proof with eauto.
-  introv. induction* A; simpl...
-Admitted.
 
  Lemma merge_double_nodup : forall l,
      nodup string_dec (merge l l) = nodup string_dec l.
@@ -1251,32 +1947,6 @@ Proof with eauto using typeindex_nodup, NoDup_nodup, merge_sorted_dedup.
       rewrite* typeindex_nodup_elim.
       Unshelve. eauto.
 Qed.
-
-Lemma nodup_empty_inv : forall l,
-    nodup string_dec l = nil -> l = nil.
-Proof.
-  introv HE. induction* l.
-  simpl in HE. case_if.
-  exfalso. forwards~: IHl. subst. inverts C.
-Qed.
-
-Lemma merge_empty_inv : forall l r,
-    merge l r = nil -> l = nil /\ r = nil.
-Proof.
-  introv HE. destruct* l; destruct* r.
-  simpl in HE. case_if.
-Qed.
-
-Lemma stype2string_toplike_complete : forall A,
-    || A || = nil -> toplike A.
-Proof with eauto.
-  introv HT. apply check_toplike_sound_complete.
-  induction A; simpl in HT; try discriminate; try case_if; simpl...
-  apply nodup_empty_inv in HT.
-  forwards (?&?): merge_empty_inv HT.
-  forwards~: IHA1. forwards~: IHA2. rewrite H1. rewrite* H2.
-Qed.
-
 Lemma stype2string_single_and_inv : forall a A B,
     [ a ] = || typ_and A B || -> ([ a ] = || A || \/ [ a ] = || B ||) /\ (nil = || A || \/ nil = || B ||).
 Proof with eauto using NoDup_nodup, merge_sorted_dedup, check_toplike_sound_complete.
@@ -1439,18 +2109,6 @@ Proof with eauto using NoDup_nodup, merge_sorted_dedup, check_toplike_sound_comp
   - admit.
 Admitted.
 
-Lemma incl_single: forall (x y : string), incl [x] [y] -> x = y.
-Proof.
-        introv HI.
-        apply incl_Forall_in_iff in HI.
-        apply Forall_inv in HI.
-        apply in_one_iff in HI. eauto.
-Qed.
-Lemma incl_eq : forall (l1 l2 : list string), l1 = l2 -> incl l1 l2.
-Proof.
-  introv Heq. rewrite Heq. applys* incl_refl.
-Qed.
-
 Lemma eqIndTyp_complete_alt_gen : forall A B,
     incl (|| B ||) (|| A ||) -> sub A B.
 Proof with eauto using NoDup_nodup, merge_sorted_dedup, check_toplike_sound_complete.
@@ -1550,41 +2208,6 @@ Admitted.
 (* (incl (nodup string_dec (syntax_ott.nsort.merge (|| a1 ||) (|| a2 ||))) ((|| a1 ||) ++ (|| a2 ||))) *)
 (* incl ((|| b1 ||) ++ (|| b2 ||)) (syntax_ott.nsort.merge (|| b1 ||) (|| b2 ||)) *)
 
-Lemma incl_eq_tindex: forall A B,
-  incl (||A||) (||B||) -> incl (||B||) (||A||) -> ||A|| = ||B||.
-Admitted.
-
-Lemma eqIndTyp_sound_alt_gen : forall A B,
-    sub A B -> incl (|| B ||) (|| A ||).
-Proof with eauto using NoDup_nodup, merge_sorted_dedup, check_toplike_sound_complete.
-  introv HS.
-  induction HS; try solve [simpl; eauto using incl_refl].
-  - rewrite* stype2string_toplike. applys incl_nil.
-  - simpl. case_if. applys incl_nil.
-    case_if. admit.
-    applys incl_eq.
-    forwards*: incl_eq_tindex A1 B1. forwards*: incl_eq_tindex A2 B2.
-    rewrite H. rewrite H0...
-  - applys incl_tran IHHS.
-    simpl. case_if. admit.
-    assert (incl ((|| A1 ||) ++ (|| A2 ||)) (nodup string_dec (syntax_ott.NSort.merge (|| A1 ||) (|| A2 ||)))) by admit.
-    applys incl_tran H.
-    applys incl_appl. applys incl_refl.
-  - admit.
-  - simpl. case_if. applys incl_nil.
-    assert (incl (nodup string_dec (syntax_ott.NSort.merge (|| A2 ||) (|| A3 ||))) ((|| A2 ||) ++ (|| A3 ||))) by admit.
-    applys incl_tran H.
-    applys* incl_app.
-Admitted.
-
-Corollary eqIndTyp_sound_alt : forall B A,
-    sub B A -> sub A B -> (|| B ||) = (|| A ||).
-Proof.
-  introv HS1 HS2.
-  apply eqIndTyp_sound_alt_gen in HS1.
-  apply eqIndTyp_sound_alt_gen in HS2.
-  (* dedup sort unique *)
-Admitted.
 
 Definition target_typ_with_same_index At Bt := exists A B, || A || = || B ||
                                                            /\ |[ A ]| = At
@@ -1598,64 +2221,8 @@ Admitted.
 (* ? directly use list in target language *)
 (* ? use a relation for type translation in target language *)
 
-(* refine subtypespec *)
-Inductive subTarget : ttyp -> ttyp -> Prop :=
- | ST_refl : forall At,
-     subTarget At At
-| ST_arrow : forall At Bt At' Bt',
-    subTarget At At' -> subTarget At' At -> subTarget Bt Bt' -> subTarget Bt' Bt -> subTarget (ttyp_arrow At Bt) (ttyp_arrow At' Bt')
- | ST_rcd : forall At Bt,
-     (forall l Ct, Tlookup l At = Some Ct -> exists Ct', Tlookup l Bt = Some Ct' /\ subTarget Ct' Ct) ->
-     subTarget Bt At.
 
-#[local] Hint Constructors subTarget : core.
 
-Lemma ST_top: forall A, subTarget |[ A ]| ttyp_top. Admitted.
-
-Lemma ST_trans: forall A B C, subTarget A B -> subTarget B C -> subTarget A C. Admitted.
-
-Lemma ST_andl : forall A B, subTarget |[ (typ_and A B) ]| |[ A ]|. Admitted.
-
-Lemma ST_andr : forall A B, subTarget |[ (typ_and A B) ]| |[ B ]|. Admitted.
-
-Lemma ST_inv : forall A B,
-    subTarget |[ A ]| |[ B ]| -> forall l Ct, Tlookup l |[ B ]| = Some Ct -> exists Ct', Tlookup l |[ A ]| = Some Ct' /\ subTarget Ct' Ct. Admitted.
-
-#[local] Hint Resolve ST_top ST_andl ST_andr : core.
-
-Lemma lookup_sub : forall A B,
-    sub A B -> subTarget |[A]| |[B]|.
-Proof.
-  introv HS.
-  induction HS; try solve [simpl; eauto].
-  - rewrite* (ttyp_trans_ord_top B)...
-  - simpl. case_if*. admit.
-    simpl. case_if*. admit.
-    +
-      rewrite* (eqIndTyp_sound_alt A1 B1). rewrite* (eqIndTyp_sound_alt A2 B2).
-      applys ST_rcd. introv HL. simpl in HL. case_if*.
-      subst. exists. split*. injection HL. intro HE. subst*.
-  - applys* ST_trans IHHS.
-  - applys* ST_trans IHHS.
-  - simpl. case_if*.
-    + applys ST_rcd. introv HL.
-      remember (Tlookup l |[A2]|). destruct o.
-      * forwards* (?&?&?): ST_inv IHHS1.
-        forwards* : lookup_concat_simpl (|[ A2 ]|) (|[ A3 ]|).
-        rewrite HL in H1. rewrite <- Heqo in H1. injection H1. intro Heq. subst*.
-      * forwards* (?&?&?): ST_inv IHHS2.
-        forwards* : lookup_concat_simpl_none (|[ A2 ]|) (|[ A3 ]|). admit.
-        rewrite* HL in H.
-Admitted.
-
-Lemma lookup_eq : forall A B,
-    subTarget A B -> subTarget B A -> forall l, Tlookup l A = None -> Tlookup l B = None.
-Proof.
-  introv HS HR.
-  induction* HS.
-  - introv HL. remember (Tlookup l At). destruct* o.
-    forwards* (?&?&?): H l. rewrite HL in H0. discriminate.
-Qed.
 
 (* Lemma lookup_sub : forall A B, *)
 (*     sub B A -> *)
